Model update

TestModels/CallingAWSSDKFromLocalService/src/SimpleCallingawssdkfromlocalserviceImpl.dfy
@@ -20,7 +20,15 @@ module SimpleCallingawssdkfromlocalserviceImpl refines AbstractSimpleCallingawss
     true
   }
 
+  predicate CallDDBGetItemEnsuresPublicly(input: CallDDBGetItemInput, output: Result<CallDDBGetItemOutput, Error>) {
+    true
+  }
+
   predicate CallKMSEncryptEnsuresPublicly(input: CallKMSEncryptInput, output: Result<CallKMSEncryptOutput, Error>) {
+    true
+  }
+
+  predicate CallKMSDecryptEnsuresPublicly(input: CallKMSDecryptInput, output: Result<CallKMSDecryptOutput, Error>) {
     true
   }
 
@@ -37,6 +45,21 @@ module SimpleCallingawssdkfromlocalserviceImpl refines AbstractSimpleCallingawss
     }
   }
 
+  method CallDDBGetItem ( config: InternalConfig,  input: CallDDBGetItemInput )
+    returns (output: Result<CallDDBGetItemOutput, Error>) {
+    var GetItemInput := Dynamodb.Types.GetItemInput(
+      TableName := input.tableArn,
+      Key := input.key
+    );
+    var retGetItem := input.ddbClient.GetItem(GetItemInput);
+    var emptyMap : Dynamodb.Types.AttributeMap := map[];
+    if retGetItem.Success? {
+      return Success(CallDDBGetItemOutput(itemOutput := retGetItem.value.Item.UnwrapOr(emptyMap)));
+    } else {
+      return Failure(ComAmazonawsDynamodb(retGetItem.error));
+    }
+  }
+
   method CallKMSEncrypt ( config: InternalConfig,  input: CallKMSEncryptInput )
     returns (output: Result<CallKMSEncryptOutput, Error>) {
     var encryptInput := Kms.Types.EncryptRequest(
@@ -49,6 +72,21 @@ module SimpleCallingawssdkfromlocalserviceImpl refines AbstractSimpleCallingawss
     var retEncryptResponse := input.kmsClient.Encrypt(encryptInput);
     if retEncryptResponse.Success? {
       return Success(CallKMSEncryptOutput(encryptOutput := retEncryptResponse.value.KeyId.UnwrapOr("DummyString")));
+    } else {
+      return Failure(Types.ComAmazonawsKms(retEncryptResponse.error));
+    }
+  }
+
+  method CallKMSDecrypt ( config: InternalConfig,  input: CallKMSDecryptInput )
+    returns (output: Result<CallKMSDecryptOutput, Error>) {
+    var decryptInput := Kms.Types.DecryptRequest(
+      CiphertextBlob := input.ciphertextBlob,
+      KeyId := Wrappers.Some(input.keyId)
+    );
+    var retEncryptResponse := input.kmsClient.Decrypt(decryptInput);
+    var emptyPlainText : Kms.Types.PlaintextType := [ 0 ];
+    if retEncryptResponse.Success? {
+      return Success(CallKMSDecryptOutput(KeyIdType := retEncryptResponse.value.KeyId.UnwrapOr("DummyString"), Plaintext := retEncryptResponse.value.Plaintext.UnwrapOr(emptyPlainText)));
     } else {
       return Failure(Types.ComAmazonawsKms(retEncryptResponse.error));
     }
